I wish I had Autosubst rn

LeanALaCarte/Test/STLC.lean
@@ -4,9 +4,22 @@ import LeanALaCarte.ExtendInd
 import LeanALaCarte.ModularCommand
 import LeanALaCarte.ModDef
 
+--Utils for later
+section
 inductive List.Has : List α → α → Type where
   | head : List.Has (a::l) a
   | tail : List.Has l a → List.Has (b::l) a
+
+abbrev Rel (α : Sort u) := α → α → Prop
+
+inductive RTC (R : Rel α) : Rel α where
+  | intro : R a b → RTC R a b
+  | refl : RTC R a a
+  | trans : R a b → RTC R b c → RTC R a c
+
+def Confluent (R : Rel α) : Prop := ∀ (a b c : α), R a b → R a c → ∃ d, RTC R b d ∧ RTC R c d
+
+end
 
 inductive Ty where
   -- Needed to avoid issue `lean4#13364` (https://github.com/leanprover/lean4/issues/13364)
@@ -17,31 +30,53 @@ set_option inductive.autoPromoteIndices false
 inductive Var  : List Ty → Ty → Type
   | var (h : Γ.Has A) : Var Γ A
 
-def Ren {T} (Γ Δ : List T) := ∀ A, Γ.Has A → Δ.Has A
+def Ren {T} (Γ Δ : List T) := ∀ A, Δ.Has A → Γ.Has A
 
 def Ren.id : Ren Γ Γ := fun _ h => h
+
+def Ren.comp (R₁ : Ren Γ₁ Γ₂) (R₂ : Ren Γ₂ Γ₃) : Ren Γ₁ Γ₃ := fun _ h => R₁ _ (R₂ _ h)
+
+infixr:90 " ∘ᵣ " => Ren.comp
 
 def Ren.ext (R : Ren Γ Δ) A: Ren (A::Γ) (A::Δ)
   | _,.head => .head
   | _,.tail h => .tail (R _ h)
 
-def Ren.wk (A) : Ren Γ (A::Γ) := fun _ h => .tail h
+theorem Ren.ext_comp_ext (R₁ : Ren Γ₁ Γ₂) (R₂ : Ren Γ₂ Γ₃) : (R₁.ext A) ∘ᵣ R₂.ext A = (R₁ ∘ᵣ R₂).ext A := by
+  funext _ h
+  cases h <;> rfl
 
-def Var.wk (R : Ren Γ Δ) : Var Γ B → Var Δ B
+def Ren.drop (A) (R : Ren Γ Δ): Ren (A::Γ) Δ := fun _ h => .tail (R _ h)
+
+def Ren.wk (A) : Ren (A::Γ) Γ := Ren.drop _ .id
+
+def Var.wk (R : Ren Γ Δ) : Var Δ B → Var Γ B
   | var h => .var (R _ h)
 
-def Var.Subst (Γ Δ : List Ty) := ∀ ⦃A⦄, Γ.Has A → Var Δ A
+theorem Var.wk_comp (R₁ : Ren Γ₁ Γ₂) (R₂ : Ren Γ₂ Γ₃) : Var.wk R₁ (Var.wk R₂ t) = Var.wk (R₁ ∘ᵣ R₂) t := by
+  induction t generalizing Γ₁ Γ₂
+  rfl
+
+def Var.Subst (Γ Δ : List Ty) := ∀ ⦃A⦄, Δ.Has A → Var Γ A
 
 def Var.Subst.id : Var.Subst Γ Γ := fun _ h => .var h
 
-def Var.subst (s : Var.Subst Γ Δ) : Var Γ A → Var Δ A
+def Var.subst (s : Var.Subst Γ Δ) : Var Δ A → Var Γ A
   | .var h => s h
+
+def Var.Subst.comp (s₁ : Var.Subst Γ₁ Γ₂) (s₂ : Var.Subst Γ₂ Γ₃) : Var.Subst Γ₁ Γ₃ :=
+  fun _ h => Var.subst s₁ (s₂ h)
 
 theorem Var.subst_id : Var.subst Var.Subst.id t = t := by
   induction t
   rfl
+theorem Var.wk_subst :
+  ∀ {Ξ Δ Γ A} (R : Ren Γ Δ) (s : Var.Subst Δ Ξ) (t : Var Ξ A),
+    Var.wk R (Var.subst (A := A) s t) = Var.subst (fun _ h => Var.wk R (s h)) t := by
+  intro Ξ Δ Γ A R s t
+  induction t generalizing Γ Δ; rfl --These generalisations are necessary for later proofs to be well-formed, any way induction proofs could be "generalized after the fact" ?
 
-inductive Var.Red : Var Γ A → Var Γ A → Prop where
+inductive Var.Step : Var Γ A → Var Γ A → Prop where
 
 modular
   inductive NatTy extends Ty where
@@ -57,6 +92,13 @@ modular
       | .const a => .const a
       | .plus a b => .plus (NatExt.wk R a) (NatExt.wk R b)
 
+  mod_def NatExt.wk_comp extends Var.wk_comp where
+    finally
+      · intros
+        simp only [NatExt.wk]
+      · intro _ _ _ a_ih b_ih _ _ _ _
+        simp [NatExt.wk,a_ih,b_ih]
+
   mod_def NatExt.Subst extends Var.Subst
 
   mod_def NatExt.subst extends Var.subst where
@@ -65,6 +107,7 @@ modular
       | .plus a b => .plus (NatExt.subst s a) (NatExt.subst s b)
 
   mod_def NatExt.Subst.id extends Var.Subst.id
+  mod_def NatExt.Subst.comp extends Var.Subst.comp
 
   mod_def NatExt.subst_id extends Var.subst_id where
     finally
@@ -72,10 +115,17 @@ modular
       · intro Γ a b a_ih b_ih
         rw [NatExt.subst,a_ih,b_ih]
 
-  inductive NatExt.Red extends Var.Red where
-    | plus_const : NatExt.Red (.plus (.const a) (.const b)) (.const (a + b))
-    | plus_lhs : NatExt.Red a₁ a₂ → NatExt.Red (.plus a₁ b) (.plus a₂ b)
-    | plus_rhs : NatExt.Red b₁ b₂ → NatExt.Red (.plus a b₁) (.plus a b₂)
+  mod_def NatExt.wk_subst extends Var.wk_subst where
+    finally
+      · intros
+        rfl
+      · intros Γ a b a_ih b_ih s
+        simp [NatExt.subst,NatExt.wk,a_ih,b_ih]
+
+  inductive NatExt.Step extends Var.Step where
+    | plus_const : NatExt.Step (.plus (.const a) (.const b)) (.const (a + b))
+    | plus_lhs : NatExt.Step a₁ a₂ → NatExt.Step (.plus a₁ b) (.plus a₂ b)
+    | plus_rhs : NatExt.Step b₁ b₂ → NatExt.Step (.plus a b₁) (.plus a b₂)
 
 modular
   inductive LamTy extends NatTy where
@@ -90,30 +140,41 @@ modular
       | _, .lam f => .lam (Term.wk (Ren.ext R _) f)
       | _, .app a b => .app (Term.wk R a) (Term.wk R b)
 
+  mod_def Term.wk_comp extends NatExt.wk_comp where
+    finally
+    · intro _ _ _ _ a_ih _ _ _ _
+      simp only [Term.wk,a_ih,Ren.ext_comp_ext]
+    · intros
+      clear Term.wk_comp
+      simp only [Term.wk, *]
+
   mod_def Term.Subst extends NatExt.Subst
   mod_def Term.Subst.id extends NatExt.Subst.id
 
-  theorem Term.wk_wk {Γ : List LamTy} {h : Γ.Has A} : Term.wk (Ren.wk B) (Subst.id A h) = (Subst.id A h.tail) := rfl
+  theorem Term.wk_id {Γ : List LamTy} {h : Γ.Has A} : Term.wk (Ren.wk B) (Subst.id A h) = (Subst.id A h.tail) := rfl
 
-  def Term.subst_ext (s : Term.Subst Γ Δ): Term.Subst (A::Γ) (A::Δ)
+  def Term.subst_ext (s : Term.Subst Γ Δ) A : Term.Subst (A::Γ) (A::Δ)
     | _ ,.head => .var .head
     | _ ,.tail h => Term.wk (Ren.wk _) (s h)
 
-  theorem Term.subst_ext_id : @Term.subst_ext Γ Γ A Term.Subst.id = Term.Subst.id := by
+  theorem Term.subst_ext_id : @Term.subst_ext Γ Γ Term.Subst.id A = Term.Subst.id := by
     funext _ h
     cases h
     · rfl
     · rw [subst_ext]
       rfl
-
-  def Term.subst_wk (a : Term Γ A) : Term.Subst (A::Γ) Γ
+  def Term.subst_wk (a : Term Γ A) : Term.Subst Γ (A::Γ)
     | _,.head => a
     | _,.tail h => .var h
 
   mod_def Term.subst extends NatExt.subst where
     match_1 with
-      | _, .lam f => .lam (Term.subst (Term.subst_ext s) f)
+      | _, .lam f => .lam (Term.subst (Term.subst_ext s _) f)
       | _, .app a b => .app (Term.subst s a) (Term.subst s b)
+
+  mod_def Term.Subst.comp extends NatExt.Subst.comp
+
+  infixr:90 " ∘ₛₜ " => Term.Subst.comp
 
   mod_def Term.subst_id extends NatExt.subst_id where
     finally
@@ -122,8 +183,47 @@ modular
       · intro _ _ _ a b a_ih b_ih
         rw [Term.subst,a_ih,b_ih]
 
-  inductive Term.Red extends NatExt.Red where
-    | beta : Term.Red (.app (.lam f) x) (Term.subst (Term.subst_wk x) f)
-    | lam : Term.Red f₁ f₂ → Term.Red (.lam f₁) (.lam f₂)
-    | app_lhs : Term.Red f₁ f₂ → Term.Red (.app f₁ x) (.app f₂ x)
-    | app_rhs : Term.Red x₁ x₂ → Term.Red (.app f x₁) (.app f x₂)
+  inductive Term.Step extends NatExt.Step where
+    | beta : Term.Step (.app (.lam f) x) (Term.subst (Term.subst_wk x) f)
+    | lam : Term.Step f₁ f₂ → Term.Step (.lam f₁) (.lam f₂)
+    | app_lhs : Term.Step f₁ f₂ → Term.Step (.app f₁ x) (.app f₂ x)
+    | app_rhs : Term.Step x₁ x₂ → Term.Step (.app f x₁) (.app f x₂)
+
+  local infixr:75 " ⤳ " => Term.Step
+  local infixr:75 " ⤳⋆ " => RTC Term.Step
+
+  mod_def Term.wk_subst extends NatExt.wk_subst where
+    finally
+    · intro A Γ B f f_ih R s _ _
+      simp [Term.subst,Term.wk,f_ih]
+      congr
+      funext x h
+      cases h
+      · rfl
+      · simp only [Term.subst_ext,Term.wk_comp]
+        rfl
+    · intro A Γ B f x ihf ihx
+      simp [Term.subst, Term.wk, ihf, ihx]
+
+  theorem Term.subst_ext_comp {Γ₁ Γ₂ Γ₃} (s₁ : Term.Subst Γ₁ Γ₂) (s₂ : Term.Subst Γ₂ Γ₃)
+    : Subst.comp (Term.subst_ext s₁ A) (Term.subst_ext s₂ A) = Term.subst_ext (s₁.comp s₂) A := by
+      funext _ h
+      cases h
+      · rfl
+      · simp [Subst.comp,subst_ext,wk_subst]
+        sorry
+
+  theorem Term.subst_comp {Γ Δ Ξ : List LamTy} :
+    ∀ {A} (t : Term Ξ A), ∀ (s₁ : Subst Γ Δ) (s₂ : Subst Δ Ξ),
+    subst s₁ (subst s₂ t) = subst (s₁.comp s₂) t := by
+      intro A t
+      induction t generalizing Γ Δ <;> intro s₁ s₂ <;> try rfl
+      case plus _ a b a_ih b_ih =>
+        simp [subst,a_ih,b_ih]
+      case lam _ _ a a_ih =>
+        rw [subst,subst,subst,a_ih,subst_ext_comp]
+      case app _ _ _ a b a_ih b_ih =>
+        simp [subst, a_ih,b_ih]
+
+
+  theorem Term.Step.Confluent : Confluent (@Term.Step Γ A) := sorry
